MonadJoin/Monad.v
@@ -4,25 +4,37 @@ Require Import HSLib.Base.
 Require Export HSLib.Functor.Functor.
 Require Export HSLib.Applicative.Applicative.
 
-(* Definition of monad using ret and join. *)
+(* Definition of monad using join. *)
 Class Monad (M : Type -> Type) : Type :=
 {
     is_applicative :> Applicative M;
     join : forall {A : Type}, M (M A) -> M A;
-    join_law :
-      forall (X : Type),
-        fmap join .> join = join .> @join X;
-    ret_law :
-      forall (X : Type),
-        ret .> join = fmap ret .> @join X;
+    join_fmap_join :
+      forall (A : Type) (x : M (M (M A))),
+        join (fmap join x) = join (join x);
     join_ret :
-      forall (A : Type) (ma : M A), join (ret ma) = ma
+      forall (A : Type) (ma : M A), join (ret ma) = ma;
+    join_fmap_ret :
+      forall (A : Type) (x : M A),
+        join (fmap ret x) = x;
+    join_fmap_fmap :
+      forall (A B : Type) (f : A -> B) (x : M (M A)),
+        join (fmap (fmap f) x) = fmap f (join x);
+    join_ap :
+      forall (A B : Type) (mf : M (A -> B)) (ma : M A),
+        mf <*> ma =
+        join (ret (fun f : A -> B => join (fmap (f .> ret) ma)) <*> mf)
 }.
 
 Coercion is_applicative : Monad >-> Applicative.
 
+Hint Rewrite @join_fmap_join @join_ret @join_fmap_ret @join_fmap_fmap
+  @join_ap : join.
+
+Ltac monad := autorewrite with join.
+
 Definition bind
-  {A B : Type} {M : Type -> Type} {inst : Monad M} (ma : M A) (f : A -> M B)
+  {M : Type -> Type} {inst : Monad M} {A B : Type} (ma : M A) (f : A -> M B)
     : M B := (fmap f .> join) ma.
 
 Definition bind_
@@ -58,13 +70,16 @@ Variable M : Type -> Type.
 Variable inst : Monad M.
 Variables A B C D E F : Type.
 
-
 Fixpoint foldM (f : A -> B -> M A) (dflt : A) (l : list B)
     : M A :=
 match l with
     | [] => ret dflt
     | h :: t => f dflt h >>= fun a : A => foldM f a t
 end.
+
+Definition ab {A B : Type} (mf : M (A -> B)) (ma : M A) : M B :=
+  mf >>= fun f =>
+  ma >>= fun a => ret (f a).
 
 End MonadicFuns.
 
@@ -76,4 +91,57 @@ Variables
   (M : Type -> Type)
   (inst : Monad M).
 
-End DerivedLaws. (* TODO *)
+Lemma bind_ret_l :
+  forall (A B : Type) (f : A -> M B) (a : A),
+    bind (ret a) f = f a.
+Proof.
+  unfold bind, compose; intros.
+  rewrite fmap_ret, join_ret. reflexivity.
+Qed.
+
+Lemma bind_ret_r :
+  forall (A : Type) (ma : M A),
+    bind ma ret = ma.
+Proof.
+  unfold bind, compose; intros.
+  rewrite join_fmap_ret. reflexivity.
+Qed.
+
+Lemma assoc :
+  forall (A B C : Type) (ma : M A) (f : A -> M B) (g : B -> M C),
+    bind (bind ma f) g = bind ma (fun x => bind (f x) g).
+Proof.
+  unfold bind, compose; intros.
+  rewrite <- !join_fmap_fmap.
+  change (fun x : A => join (fmap g (f x))) with (f .> fmap g .> join).
+  rewrite !fmap_pres_comp. unfold compose. rewrite join_fmap_join.
+  reflexivity.
+Qed.
+
+Lemma bind_fmap :
+  forall (A B C : Type) (f : A -> B) (x : M A) (g : B -> M C),
+    bind (fmap f x) g = bind x (f .> g).
+Proof.
+  unfold bind, compose, id; intros. f_equal.
+  rewrite <- fmap_pres_comp'. unfold compose.
+  reflexivity.
+Qed.
+
+Lemma fmap_bind :
+  forall (A B C : Type) (x : M A) (f : A -> M B) (g : B -> C),
+    fmap g (bind x f) = bind x (fun x0 : A => fmap g (f x0)).
+Proof.
+  intros. change (fun x0 : A => fmap g (f x0)) with (f .> fmap g).
+  rewrite <- bind_fmap. unfold bind, compose; intros.
+  rewrite join_fmap_fmap. reflexivity.
+Qed.
+
+Lemma bind_ap :
+  forall (A B : Type) (mf : M (A -> B)) (mx : M A),
+    ap mf mx = bind mf (fun f => bind mx (fun x => ret (f x))).
+Proof.
+  intros. unfold bind, compose. rewrite join_ap. applicative.
+  unfold compose. reflexivity.
+Qed.
+
+End DerivedLaws.
